ulib/FStar.Stubs.Tactics.Types.fsti
@@ -62,10 +62,10 @@ type guard_policy =
     | Drop      // Drop guards, clearly unsound! careful!
 
 (* Typing reflection *)
-val non_informative_token (g:env) (t:typ) : Type0
-val subtyping_token (g:env) (t0 t1:typ) : Type0
-val equiv_token (g:env) (t0 t1:typ) : Type0
-val typing_token (g:env) (e:term) (c:tot_or_ghost & typ) : Type0
+[@@ erasable] val non_informative_token (g:env) (t:typ) : Type0
+[@@ erasable] val subtyping_token (g:env) (t0 t1:typ) : Type0
+[@@ erasable] val equiv_token (g:env) (t0 t1:typ) : Type0
+[@@ erasable] val typing_token (g:env) (e:term) (c:tot_or_ghost & typ) : Type0
 
 (* Must be inline, this definition is not there in src/FStar.Tactics.Types *)
 inline_for_extraction
